Include a typing judgment for values so we can type check definitions.

theories/fundamental.v
@@ -28,43 +28,69 @@ Section fundamental.
     ty_bin_op op τ1 τ2 σ → SemTyBinOp op (⟦ τ1 ⟧ ρ) (⟦ τ2 ⟧ ρ) (⟦ σ ⟧ ρ).
   Proof. destruct 1; simpl; apply _. Qed.
 
-  Theorem fundamental Γ e τ ρ :
-    (Γ ⊢ₜ e : τ) →
-    interp_env Γ ρ ⊨ e : ⟦ τ ⟧ ρ.
+  Fixpoint fundamental Γ e τ ρ (Hty : Γ ⊢ₜ e : τ) : interp_env Γ ρ ⊨ e : ⟦ τ ⟧ ρ
+  with fundamental_val v τ ρ (Hty : ⊢ᵥ v : τ) : ⊨ᵥ v : ⟦ τ ⟧ ρ.
   Proof.
-    intros Htyped. iInduction Htyped as [] "IH" forall (ρ); simpl in *.
-    - iApply Var_sem_typed. by apply lookup_interp_env.
-    - iApply Unit_sem_typed.
-    - iApply Bool_sem_typed.
-    - iApply Int_sem_typed.
-    - by iApply Pair_sem_typed.
-    - by iApply Fst_sem_typed.
-    - by iApply Snd_sem_typed.
-    - by iApply InjL_sem_typed.
-    - by iApply InjR_sem_typed.
-    - by iApply Case_sem_typed.
-    - iApply Rec_sem_typed. iSpecialize ("IH" $! ρ).
-      by rewrite !interp_env_binder_insert.
-    - by iApply App_sem_typed.
-    - iApply TLam_sem_typed; iIntros (A). iSpecialize ("IH" $! (A :: ρ)).
-      by rewrite interp_env_ty_lift /=; last lia.
-    - rewrite interp_ty_subst /=; last lia.
-      iApply (TApp_sem_typed with "IH").
-    - iApply Pack_sem_typed. iSpecialize ("IH" $! ρ).
-      by rewrite interp_ty_subst; last lia.
-    - iApply (Unpack_sem_typed with "IH"); iIntros (A).
-      iSpecialize ("IH1" $! (A :: ρ)).
-      rewrite interp_env_binder_insert.
-      rewrite interp_env_ty_lift /=; last lia.
-      by rewrite interp_ty_lift /=; last lia.
-    - by iApply Alloc_sem_typed.
-    - by iApply Load_sem_typed.
-    - by iApply Store_sem_typed.
-    - by iApply FAA_sem_typed.
-    - by iApply CmpXchg_sem_typed.
-    - by iApply UnOp_sem_typed.
-    - by iApply BinOp_sem_typed.
-    - by iApply If_sem_typed.
-    - by iApply Fork_sem_typed.
-  Qed.
+    - destruct Hty; simpl.
+      + iApply Var_sem_typed. by apply lookup_interp_env.
+      + iApply Val_sem_typed; by iApply fundamental_val.
+      + iApply Pair_sem_typed; by iApply fundamental.
+      + iApply Fst_sem_typed; by iApply (fundamental _ _ (_ * _)%ty).
+      + iApply Snd_sem_typed; by iApply (fundamental _ _ (_ * _)%ty).
+      + iApply InjL_sem_typed; by iApply fundamental.
+      + iApply InjR_sem_typed; by iApply fundamental.
+      + iApply Case_sem_typed.
+        * by iApply (fundamental _ _ (_ + _)%ty).
+        * by iApply (fundamental _ _ (_ → _)%ty).
+        * by iApply (fundamental _ _ (_ → _)%ty).
+      + iApply Rec_sem_typed.
+        change (⟦ ?τ1 ⟧ _ → ⟦ ?τ2 ⟧ _)%sem_ty with (⟦ τ1 → τ2 ⟧ ρ).
+        rewrite -!interp_env_binder_insert. by iApply fundamental.
+      + iApply App_sem_typed.
+        * by iApply (fundamental _ _ (_ → _)%ty).
+        * by iApply fundamental.
+      + iApply TLam_sem_typed; iIntros (A).
+        rewrite -interp_env_ty_lift_0. by iApply fundamental.
+      + rewrite interp_ty_subst_0.
+        iApply (TApp_sem_typed _ _ (λ A, ⟦ _ ⟧ (A :: _))).
+        by iApply (fundamental _ _ (∀: _)%ty).
+      + iApply (Pack_sem_typed _ _ _ (⟦ _ ⟧ ρ)).
+        rewrite -interp_ty_subst_0. by iApply fundamental.
+      + iApply (Unpack_sem_typed _ _ _ _ (λ A, ⟦ _ ⟧ (A :: _))).
+        * by iApply (fundamental _ _ (∃: _)%ty).
+        * iIntros (A).
+          rewrite -(interp_ty_lift_0 _ A ρ) -(interp_env_ty_lift_0 _ A ρ).
+          rewrite -interp_env_binder_insert.
+          by iApply fundamental.
+      + iApply Alloc_sem_typed. by iApply fundamental.
+      + iApply Load_sem_typed. by iApply (fundamental _ _ (ref _)%ty).
+      + iApply Store_sem_typed.
+        * by iApply (fundamental _ _ (ref _)%ty).
+        * by iApply fundamental.
+      + iApply FAA_sem_typed.
+        * by iApply (fundamental _ _ (ref TInt)%ty).
+        * by iApply (fundamental _ _ TInt).
+      + iApply CmpXchg_sem_typed.
+        * by iApply (fundamental _ _ (ref _)%ty).
+        * by iApply fundamental.
+        * by iApply fundamental.
+      + iApply UnOp_sem_typed. by iApply fundamental.
+      + iApply BinOp_sem_typed; by iApply fundamental.
+      + iApply If_sem_typed.
+        * by iApply (fundamental _ _ TBool).
+        * by iApply fundamental.
+        * by iApply fundamental.
+      + iApply Fork_sem_typed. by iApply (fundamental _ _ TUnit).
+    - destruct Hty; simpl.
+      + iApply UnitV_sem_typed.
+      + iApply BoolV_sem_typed.
+      + iApply IntV_sem_typed.
+      + iApply PairV_sem_typed; by iApply fundamental_val.
+      + iApply InjLV_sem_typed; by iApply fundamental_val.
+      + iApply InjRV_sem_typed; by iApply fundamental_val.
+      + iApply RecV_sem_typed.
+        change (⟦ ?τ1 ⟧ _ → ⟦ ?τ2 ⟧ _)%sem_ty with (⟦ τ1 → τ2 ⟧ ρ).
+        rewrite -(interp_env_empty ρ) -!interp_env_binder_insert.
+        by iApply fundamental.
+   Qed.
 End fundamental.
