theories/typed.v
@@ -29,89 +29,111 @@ Existing Class ty_bin_op.
 Existing Instances Ty_bin_op_eq Ty_bin_op_arith Ty_bin_op_compare Ty_bin_op_bool.
 
 Reserved Notation "Γ ⊢ₜ e : τ" (at level 74, e, τ at next level).
-Inductive typed (Γ : gmap string ty) : expr → ty → Prop :=
+Reserved Notation "⊢ᵥ v : τ" (at level 20, v, τ at next level).
+
+Inductive typed : gmap string ty → expr → ty → Prop :=
   (** Variables *)
-  | Var_typed x τ :
+  | Var_typed Γ x τ :
      Γ !! x = Some τ →
      Γ ⊢ₜ Var x : τ
-  (** Base tys *)
-  | Unit_typed :
-     Γ ⊢ₜ #() : TUnit
-  | Bool_typed (b : bool) :
-     Γ ⊢ₜ # b : TBool
-  | Int_typed (i : Z) :
-     Γ ⊢ₜ # i : TInt
+  (** Values *)
+  | Val_typed Γ v τ :
+     val_typed v τ →
+     Γ ⊢ₜ v : τ
   (** Products and sums *)
-  | Pair_typed e1 e2 τ1 τ2 :
+  | Pair_typed Γ e1 e2 τ1 τ2 :
      Γ ⊢ₜ e1 : τ1 → Γ ⊢ₜ e2 : τ2 →
      Γ ⊢ₜ Pair e1 e2 : TProd τ1 τ2
-  | Fst_typed e τ1 τ2 :
+  | Fst_typed Γ e τ1 τ2 :
      Γ ⊢ₜ e : TProd τ1 τ2 →
      Γ ⊢ₜ Fst e : τ1
-  | Snd_typed e τ1 τ2 :
+  | Snd_typed Γ e τ1 τ2 :
      Γ ⊢ₜ e : TProd τ1 τ2 →
      Γ ⊢ₜ Snd e : τ2
-  | InjL_typed e τ1 τ2 :
+  | InjL_typed Γ e τ1 τ2 :
      Γ ⊢ₜ e : τ1 →
      Γ ⊢ₜ InjL e : TSum τ1 τ2
-  | InjR_typed e τ1 τ2 :
+  | InjR_typed Γ e τ1 τ2 :
      Γ ⊢ₜ e : τ2 →
      Γ ⊢ₜ InjR e : TSum τ1 τ2
-  | Case_typed e0 e1 e2 τ1 τ2 τ3 :
+  | Case_typed Γ e0 e1 e2 τ1 τ2 τ3 :
      Γ ⊢ₜ e0 : TSum τ1 τ2 → Γ ⊢ₜ e1 : TArr τ1 τ3 → Γ ⊢ₜ e2 : TArr τ2 τ3 →
      Γ ⊢ₜ Case e0 e1 e2 : τ3
   (** Functions *)
-  | Rec_typed f x e τ1 τ2 :
+  | Rec_typed Γ f x e τ1 τ2 :
      binder_insert f (TArr τ1 τ2) (binder_insert x τ1 Γ) ⊢ₜ e : τ2 →
      Γ ⊢ₜ Rec f x e : TArr τ1 τ2
-  | App_typed e1 e2 τ1 τ2 :
+  | App_typed Γ e1 e2 τ1 τ2 :
      Γ ⊢ₜ e1 : TArr τ1 τ2 → Γ ⊢ₜ e2 : τ1 →
      Γ ⊢ₜ App e1 e2 : τ2
   (** Polymorphic functions and existentials *)
-  | TLam_typed e τ :
+  | TLam_typed Γ e τ :
      ty_lift 0 <$> Γ ⊢ₜ e : τ →
      Γ ⊢ₜ (Λ: e) : TForall τ
-  | TApp_typed e τ τ' :
+  | TApp_typed Γ e τ τ' :
      Γ ⊢ₜ e : TForall τ →
      Γ ⊢ₜ e <_> : ty_subst 0 τ' τ
-  | Pack_typed e τ τ' :
+  | Pack_typed Γ e τ τ' :
      Γ ⊢ₜ e : ty_subst 0 τ' τ →
      Γ ⊢ₜ e : TExist τ
-  | Unpack_typed e1 x e2 τ τ2 :
+  | Unpack_typed Γ e1 x e2 τ τ2 :
      Γ ⊢ₜ e1 : TExist τ →
      binder_insert x τ (ty_lift 0 <$> Γ) ⊢ₜ e2 : ty_lift 0 τ2 →
      Γ ⊢ₜ (unpack: x := e1 in e2) : τ2
   (** Heap operations *)
-  | Alloc_typed e τ :
+  | Alloc_typed Γ e τ :
      Γ ⊢ₜ e : τ →
      Γ ⊢ₜ Alloc e : TRef τ
-  | Load_typed e τ :
+  | Load_typed Γ e τ :
      Γ ⊢ₜ e : TRef τ →
      Γ ⊢ₜ Load e : τ
-  | Store_typed e1 e2 τ :
+  | Store_typed Γ e1 e2 τ :
      Γ ⊢ₜ e1 : TRef τ → Γ ⊢ₜ e2 : τ →
      Γ ⊢ₜ Store e1 e2 : TUnit
-  | FAA_typed e1 e2 :
+  | FAA_typed Γ e1 e2 :
      Γ ⊢ₜ e1 : TRef TInt → Γ ⊢ₜ e2 : TInt →
      Γ ⊢ₜ FAA e1 e2 : TInt
-  | CmpXchg_typed e1 e2 e3 τ :
+  | CmpXchg_typed Γ e1 e2 e3 τ :
      ty_unboxed τ →
      Γ ⊢ₜ e1 : TRef τ → Γ ⊢ₜ e2 : τ → Γ ⊢ₜ e3 : τ →
      Γ ⊢ₜ CmpXchg e1 e2 e3 : TProd τ TBool
   (** Operators *)
-  | UnOp_typed op e τ σ :
+  | UnOp_typed Γ op e τ σ :
      Γ ⊢ₜ e : τ →
      ty_un_op op τ σ →
      Γ ⊢ₜ UnOp op e : σ
-  | BinOp_typed op e1 e2 τ1 τ2 σ :
+  | BinOp_typed Γ op e1 e2 τ1 τ2 σ :
      Γ ⊢ₜ e1 : τ1 → Γ ⊢ₜ e2 : τ2 →
      ty_bin_op op τ1 τ2 σ →
      Γ ⊢ₜ BinOp op e1 e2 : σ
-  | If_typed e0 e1 e2 τ :
+  | If_typed Γ e0 e1 e2 τ :
      Γ ⊢ₜ e0 : TBool → Γ ⊢ₜ e1 : τ → Γ ⊢ₜ e2 : τ →
      Γ ⊢ₜ If e0 e1 e2 : τ
   (** Fork *)
-  | Fork_typed e :
+  | Fork_typed Γ e :
      Γ ⊢ₜ e : TUnit →
      Γ ⊢ₜ Fork e : TUnit
-where "Γ ⊢ₜ e : τ" := (typed Γ e τ).
+with val_typed : val → ty → Prop :=
+  (** Base types *)
+  | UnitV_typed :
+     ⊢ᵥ #() : TUnit
+  | BoolV_typed (b : bool) :
+     ⊢ᵥ #b : TBool
+  | IntV_val_typed (i : Z) :
+     ⊢ᵥ #i : TInt
+  (** Products and sums *)
+  | PairV_typed v1 v2 τ1 τ2 :
+     ⊢ᵥ v1 : τ1 → ⊢ᵥ v2 : τ2 →
+     ⊢ᵥ PairV v1 v2 : TProd τ1 τ2
+  | InjLV_typed v τ1 τ2 :
+     ⊢ᵥ v : τ1 →
+     ⊢ᵥ InjLV v : TSum τ1 τ2
+  | InjRV_typed v τ1 τ2 :
+     ⊢ᵥ v : τ2 →
+     ⊢ᵥ InjRV v : TSum τ1 τ2
+  (** Functions *)
+  | RecV_typed f x e τ1 τ2 :
+     binder_insert f (TArr τ1 τ2) (binder_insert x τ1 ∅) ⊢ₜ e : τ2 →
+     ⊢ᵥ RecV f x e : TArr τ1 τ2
+where "Γ ⊢ₜ e : τ" := (typed Γ e τ)
+and "⊢ᵥ v : τ" := (val_typed v τ).
